Pull constructor out of monitor and make reasoning with [is_monP] easier to follow.

theories/heap_lang/lib/monitor.v
@@ -1,4 +1,5 @@
 From iris.heap_lang Require Export heap.
+From iris.heap_lang.lib Require Export constructor.
 From iris.heap_lang Require notation.
 
 (* Minor annoyance: [solve_proper] can't handle our goals. *)
@@ -13,23 +14,6 @@ Ltac apply_eq :=
 Ltac solve_proper_eq :=
   preprocess_solve_proper;
   repeat (f_equiv; try (eassumption || apply_eq)).
-
-(** * Value constructors *)
-
-Class constructor (A : Type) := Ctor {
-  ctor : A → val;
-  ctor_inj : Inj (=) (=) ctor
-}.
-
-Existing Instance ctor_inj.
-Arguments Ctor {_} _ _.
-
-Instance val_ctor : constructor val := Ctor id id_inj.
-
-Lemma locv_inj : Inj (=) (=) LocV. Proof. by move=>?? [] ->. Qed.
-Instance loc_constructor : constructor loc := Ctor LocV locv_inj.
-
-Coercion ctor : constructor >-> Funclass.
 
 (** * Reference monitors *)
 (**
@@ -60,7 +44,7 @@ Section is_mon.
 End is_mon.
 Typeclasses Opaque is_mon.
 
-(** * Reference monitors *)
+(** * Predicate-based reference monitors *)
 (**
 	The assertion [is_monP v Ψ1 Ψ2] means that [v] is a reference
 	monitor of "type" [Ψ1 → Ψ2] where [Ψ1] and [Ψ2] are predicates
@@ -74,23 +58,9 @@ Section is_monP.
   Context `{heapG Σ, fA : constructor A, fB : constructor B}.
 
   Definition is_monP (v : val) (Ψ1 : A → iProp Σ)
-      (Ψ2 : B → iProp Σ) : iProp Σ :=
-    (∀ a, {{{ Ψ1 a }}} v (fA a) ?{{{ b, RET fB b; Ψ2 b }}})%I.
+      (Ψ2 : B → iProp Σ) : iProp Σ := is_mon v Ψ1 (λ _, Ψ2).
 
-  Global Instance is_monP_persistent v Ψ1 Ψ2 :
-    PersistentP (is_monP v Ψ1 Ψ2).
-  Proof. apply _. Qed.
-
-  Global Instance is_monP_ne v n :
-     Proper (ext (dist n) ==> ext (dist n) ==> dist n) (is_monP v).
-  Proof. solve_proper. Qed.
-
-  Global Instance is_monP_proper v :
-     Proper (ext (≡) ==> ext (≡) ==> (≡)) (is_monP v).
-  Proof. solve_proper. Qed.
-
-  Lemma is_monP_rel v Ψ1 Ψ2 :
-    is_monP v Ψ1 Ψ2 ⊣⊢ is_mon v Ψ1 (λ _, Ψ2).
+  Lemma monP_triple v Ψ1 Ψ2 :
+    is_monP v Ψ1 Ψ2 ⊣⊢ (∀ a, {{{ Ψ1 a }}} v (fA a) ?{{{ b, RET fB b; Ψ2 b }}})%I.
   Proof. by []. Qed.
 End is_monP.
-Typeclasses Opaque is_monP.
