theories/heap_lang/lib/constructor.v
@@ -1,0 +1,23 @@
+From iris.heap_lang Require Export lang.
+
+(** * Value constructors *)
+(**
+	The point of these instances is to leave implicit the
+	injections into values we need to specify, say, finite maps
+	implemented in the heap language.
+*)
+
+Class constructor (A : Type) := Ctor {
+  ctor : A → val;
+  ctor_inj : Inj (=) (=) ctor
+}.
+
+Existing Instance ctor_inj.
+Arguments Ctor {_} _ _.
+
+Instance val_ctor : constructor val := Ctor id id_inj.
+
+Lemma locv_inj : Inj (=) (=) LocV. Proof. by move=>?? [] ->. Qed.
+Instance loc_constructor : constructor loc := Ctor LocV locv_inj.
+
+Coercion ctor : constructor >-> Funclass.
